Consistently use "t" instead of "ty" in Lib.Buffer for the buffer type

lib/Lib.Buffer.fsti
@@ -27,8 +27,8 @@ type buftype =
   | CONST
 
 inline_for_extraction
-let buffer_t (ty:buftype) (a:Type0) =
-  match ty with
+let buffer_t (t:buftype) (a:Type0) =
+  match t with
   | IMMUT -> IB.ibuffer a
   | MUT -> B.buffer a
   | CONST -> CB.const_buffer a
@@ -65,8 +65,8 @@ let const_to_ibuffer #a (b:cbuffer a{CB.qual_of b == CB.IMMUTABLE}) : r:ibuffer 
 
 
 inline_for_extraction
-let lbuffer_t (ty:buftype) (a:Type0) (len:size_t) =
-  b:buffer_t ty a{length #ty #a b == v len}
+let lbuffer_t (t:buftype) (a:Type0) (len:size_t) =
+  b:buffer_t t a{length #t #a b == v len}
 
 unfold let lbuffer (a:Type0) (len:size_t) = lbuffer_t MUT a len
 unfold let ilbuffer (a:Type0) (len:size_t) = lbuffer_t IMMUT a len
@@ -79,14 +79,14 @@ let const_to_lbuffer #a #len (b:clbuffer a len{CB.qual_of (b <: cbuffer a) == CB
 let const_to_ilbuffer #a #len (b:glbuffer a len)  : r:ilbuffer a len =
   const_to_ibuffer #a b
 
-unfold let null (#ty : buftype) (a : Type0) : buffer_t ty a =
-  match ty with
+unfold let null (#t : buftype) (a : Type0) : buffer_t t a =
+  match t with
   | IMMUT -> IB.inull #a
   | MUT -> B.null #a
   | CONST -> CB.null a
 
-let g_is_null (#ty : buftype) (#a : Type0) (b : buffer_t ty a) : GTot bool =
-  match ty with
+let g_is_null (#t : buftype) (#a : Type0) (b : buffer_t t a) : GTot bool =
+  match t with
   | IMMUT -> IB.g_is_null (b <: ibuffer a)
   | MUT -> B.g_is_null (b <: buffer a)
   | CONST -> B.g_is_null (CB.as_mbuf (b <: cbuffer a))
@@ -97,8 +97,8 @@ let live (#t:buftype) (#a:Type0) (h:HS.mem) (b:buffer_t t a) : Type =
   | IMMUT -> IB.live h (b <: ibuffer a)
   | CONST -> CB.live h (b <: cbuffer a)
 
-let freeable (#ty : buftype) (#a : Type0) (b : buffer_t ty a) : GTot Type0 =
-  match ty with
+let freeable (#t : buftype) (#a : Type0) (b : buffer_t t a) : GTot Type0 =
+  match t with
   | IMMUT -> IB.freeable (b <: ibuffer a)
   | MUT -> B.freeable (b <: buffer a)
   | CONST -> B.freeable (CB.as_mbuf (b <: cbuffer a))
@@ -109,25 +109,25 @@ let loc (#t:buftype) (#a:Type0) (b:buffer_t t a) : GTot B.loc =
   | IMMUT -> B.loc_buffer (b <: ibuffer a)
   | CONST -> CB.loc_buffer (b <: cbuffer a)
 
-let loc_addr_of_buffer (#ty : buftype) (#a : Type0) (b : buffer_t ty a) : GTot B.loc =
-  match ty with
+let loc_addr_of_buffer (#t : buftype) (#a : Type0) (b : buffer_t t a) : GTot B.loc =
+  match t with
   | IMMUT -> IB.loc_addr_of_buffer (b <: ibuffer a)
   | MUT -> B.loc_addr_of_buffer (b <: buffer a)
   | CONST -> B.loc_addr_of_buffer (CB.as_mbuf (b <: cbuffer a))
 
 inline_for_extraction noextract
-let is_null (#ty : buftype) (#a : Type0) (b : buffer_t ty a) :
+let is_null (#t : buftype) (#a : Type0) (b : buffer_t t a) :
   Stack bool
   (requires (fun h -> live h b))
   (ensures  (fun h y h' -> h == h' /\ y == g_is_null b)) =
-  match ty with
+  match t with
   | IMMUT -> IB.is_null (b <: ibuffer a)
   | MUT -> B.is_null (b <: buffer a)
   | CONST -> CB.is_null (b <: cbuffer a)
 
-let get (#ty : buftype) (#a : Type0) (h : mem) (b : buffer_t ty a) (i : nat{i < length b}) :
+let get (#t : buftype) (#a : Type0) (h : mem) (b : buffer_t t a) (i : nat{i < length b}) :
   GTot a =
-  match ty with
+  match t with
   | IMMUT -> IB.get h (b <: ibuffer a) i
   | MUT -> B.get h (b <: buffer a) i
   | CONST -> B.get h (CB.as_mbuf (b <: cbuffer a)) i
